Source/DafnyCore/Verifier/BoogieGenerator.ExpressionWellformed.cs
@@ -1665,7 +1665,7 @@ namespace Microsoft.Dafny {
         Cons(TypeToTy(sourceType.Result),
           Cons(etran.HeapExpr,
             Cons(etran.TrExpr(init),
-              indices.ConvertAll(idx => (Bpl.Expr)FunctionCall(tok, BuiltinFunction.Box, null, idx))))));
+              indices.ConvertAll(idx => (Bpl.Expr)ApplyBox(tok, idx))))));
       // check precond
       var pre = FunctionCall(tok, Requires(dims.Count), Bpl.Type.Bool, args);
       var q = new Bpl.ForallExpr(tok, bvs, BplImp(ante, pre));
