Source/IntegrationTests/TestFiles/LitTests/LitTest/referrers/referrers.bpl
@@ -4287,6 +4287,7 @@ implementation {:smt_option "smt.arith.solver", "2"} {:verboseName "ObjectFields
   var $nw: ref;
   var chained_test##0: ref;
   var newtype$check#0: ref;
+  var $oldRhs: ref;
   var $rhs#0: ref;
   var $rhs#1: ref;
   var $rhs#2: ref;
@@ -4372,11 +4373,29 @@ implementation {:smt_option "smt.arith.solver", "2"} {:verboseName "ObjectFields
     assume true;
     assume true;
     assert {:id "id82"} $_ModifiesFrame[t#0, _module.ChainingObject.x];
-    havoc $ReferrersHeap;
+    $oldRhs := $Unbox(read($Heap, t#0, _module.ChainingObject.x)): ref;
+    if ($oldRhs != null)
+    {
+        $ReferrersHeap := updateReferrers($ReferrersHeap, 
+          $oldRhs, 
+          Set#Difference(readReferrers($ReferrersHeap, $oldRhs), 
+            Set#UnionOne(Set#Empty(): Set, 
+              $Box(#_System._tuple#2._#Make2($Box(t#0), $Box(_module.ChainingObject.x))))));
+    }
+
     assert {:id "id83"} defass#t#0;
     assume true;
     $rhs#0 := t#0;
-    havoc $ReferrersHeap;
+    if ($rhs#0 != null)
+    {
+        assume !Set#IsMember(readReferrers($ReferrersHeap, $rhs#0), 
+          $Box(#_System._tuple#2._#Make2($Box(t#0), $Box(_module.ChainingObject.x))));
+        $ReferrersHeap := updateReferrers($ReferrersHeap, 
+          $rhs#0, 
+          Set#UnionOne(readReferrers($ReferrersHeap, $rhs#0), 
+            $Box(#_System._tuple#2._#Make2($Box(t#0), $Box(_module.ChainingObject.x)))));
+    }
+
     $Heap := update($Heap, t#0, _module.ChainingObject.x, $Box($rhs#0));
     assume $IsGoodHeap($Heap);
     assume {:captureState "referrers.dfy(118,10)"} true;
@@ -4394,11 +4413,29 @@ implementation {:smt_option "smt.arith.solver", "2"} {:verboseName "ObjectFields
     assume true;
     assume true;
     assert {:id "id91"} $_ModifiesFrame[t#0, _module.ChainingObject.y];
-    havoc $ReferrersHeap;
+    $oldRhs := $Unbox(read($Heap, t#0, _module.ChainingObject.y)): ref;
+    if ($oldRhs != null)
+    {
+        $ReferrersHeap := updateReferrers($ReferrersHeap, 
+          $oldRhs, 
+          Set#Difference(readReferrers($ReferrersHeap, $oldRhs), 
+            Set#UnionOne(Set#Empty(): Set, 
+              $Box(#_System._tuple#2._#Make2($Box(t#0), $Box(_module.ChainingObject.y))))));
+    }
+
     assert {:id "id92"} defass#t#0;
     assume true;
     $rhs#1 := t#0;
-    havoc $ReferrersHeap;
+    if ($rhs#1 != null)
+    {
+        assume !Set#IsMember(readReferrers($ReferrersHeap, $rhs#1), 
+          $Box(#_System._tuple#2._#Make2($Box(t#0), $Box(_module.ChainingObject.y))));
+        $ReferrersHeap := updateReferrers($ReferrersHeap, 
+          $rhs#1, 
+          Set#UnionOne(readReferrers($ReferrersHeap, $rhs#1), 
+            $Box(#_System._tuple#2._#Make2($Box(t#0), $Box(_module.ChainingObject.y)))));
+    }
+
     $Heap := update($Heap, t#0, _module.ChainingObject.y, $Box($rhs#1));
     assume $IsGoodHeap($Heap);
     assume {:captureState "referrers.dfy(120,10)"} true;
@@ -4418,11 +4455,29 @@ implementation {:smt_option "smt.arith.solver", "2"} {:verboseName "ObjectFields
     assume true;
     assume true;
     assert {:id "id101"} $_ModifiesFrame[t#0, _module.ChainingObject.x];
-    havoc $ReferrersHeap;
+    $oldRhs := $Unbox(read($Heap, t#0, _module.ChainingObject.x)): ref;
+    if ($oldRhs != null)
+    {
+        $ReferrersHeap := updateReferrers($ReferrersHeap, 
+          $oldRhs, 
+          Set#Difference(readReferrers($ReferrersHeap, $oldRhs), 
+            Set#UnionOne(Set#Empty(): Set, 
+              $Box(#_System._tuple#2._#Make2($Box(t#0), $Box(_module.ChainingObject.x))))));
+    }
+
     newtype$check#1 := null;
     assume true;
     $rhs#2 := null;
-    havoc $ReferrersHeap;
+    if ($rhs#2 != null)
+    {
+        assume !Set#IsMember(readReferrers($ReferrersHeap, $rhs#2), 
+          $Box(#_System._tuple#2._#Make2($Box(t#0), $Box(_module.ChainingObject.x))));
+        $ReferrersHeap := updateReferrers($ReferrersHeap, 
+          $rhs#2, 
+          Set#UnionOne(readReferrers($ReferrersHeap, $rhs#2), 
+            $Box(#_System._tuple#2._#Make2($Box(t#0), $Box(_module.ChainingObject.x)))));
+    }
+
     $Heap := update($Heap, t#0, _module.ChainingObject.x, $Box($rhs#2));
     assume $IsGoodHeap($Heap);
     assume {:captureState "referrers.dfy(122,13)"} true;
@@ -4440,11 +4495,29 @@ implementation {:smt_option "smt.arith.solver", "2"} {:verboseName "ObjectFields
     assume true;
     assume true;
     assert {:id "id109"} $_ModifiesFrame[t#0, _module.ChainingObject.y];
-    havoc $ReferrersHeap;
+    $oldRhs := $Unbox(read($Heap, t#0, _module.ChainingObject.y)): ref;
+    if ($oldRhs != null)
+    {
+        $ReferrersHeap := updateReferrers($ReferrersHeap, 
+          $oldRhs, 
+          Set#Difference(readReferrers($ReferrersHeap, $oldRhs), 
+            Set#UnionOne(Set#Empty(): Set, 
+              $Box(#_System._tuple#2._#Make2($Box(t#0), $Box(_module.ChainingObject.y))))));
+    }
+
     newtype$check#2 := null;
     assume true;
     $rhs#3 := null;
-    havoc $ReferrersHeap;
+    if ($rhs#3 != null)
+    {
+        assume !Set#IsMember(readReferrers($ReferrersHeap, $rhs#3), 
+          $Box(#_System._tuple#2._#Make2($Box(t#0), $Box(_module.ChainingObject.y))));
+        $ReferrersHeap := updateReferrers($ReferrersHeap, 
+          $rhs#3, 
+          Set#UnionOne(readReferrers($ReferrersHeap, $rhs#3), 
+            $Box(#_System._tuple#2._#Make2($Box(t#0), $Box(_module.ChainingObject.y)))));
+    }
+
     $Heap := update($Heap, t#0, _module.ChainingObject.y, $Box($rhs#3));
     assume $IsGoodHeap($Heap);
     assume {:captureState "referrers.dfy(124,13)"} true;
@@ -4460,11 +4533,29 @@ implementation {:smt_option "smt.arith.solver", "2"} {:verboseName "ObjectFields
     assume true;
     assume true;
     assert {:id "id116"} $_ModifiesFrame[t#0, _module.ChainingObject.tracking];
-    havoc $ReferrersHeap;
+    $oldRhs := $Unbox(read($Heap, t#0, _module.ChainingObject.tracking)): ref;
+    if ($oldRhs != null)
+    {
+        $ReferrersHeap := updateReferrers($ReferrersHeap, 
+          $oldRhs, 
+          Set#Difference(readReferrers($ReferrersHeap, $oldRhs), 
+            Set#UnionOne(Set#Empty(): Set, 
+              $Box(#_System._tuple#2._#Make2($Box(t#0), $Box(_module.ChainingObject.tracking))))));
+    }
+
     assert {:id "id117"} defass#t#0;
     assume true;
     $rhs#4 := t#0;
-    havoc $ReferrersHeap;
+    if ($rhs#4 != null)
+    {
+        assume !Set#IsMember(readReferrers($ReferrersHeap, $rhs#4), 
+          $Box(#_System._tuple#2._#Make2($Box(t#0), $Box(_module.ChainingObject.tracking))));
+        $ReferrersHeap := updateReferrers($ReferrersHeap, 
+          $rhs#4, 
+          Set#UnionOne(readReferrers($ReferrersHeap, $rhs#4), 
+            $Box(#_System._tuple#2._#Make2($Box(t#0), $Box(_module.ChainingObject.tracking)))));
+    }
+
     $Heap := update($Heap, t#0, _module.ChainingObject.tracking, $Box($rhs#4));
     assume $IsGoodHeap($Heap);
     assume {:captureState "referrers.dfy(126,17)"} true;
@@ -4482,11 +4573,29 @@ implementation {:smt_option "smt.arith.solver", "2"} {:verboseName "ObjectFields
     assume true;
     assume true;
     assert {:id "id125"} $_ModifiesFrame[t#0, _module.ChainingObject.tracking];
-    havoc $ReferrersHeap;
+    $oldRhs := $Unbox(read($Heap, t#0, _module.ChainingObject.tracking)): ref;
+    if ($oldRhs != null)
+    {
+        $ReferrersHeap := updateReferrers($ReferrersHeap, 
+          $oldRhs, 
+          Set#Difference(readReferrers($ReferrersHeap, $oldRhs), 
+            Set#UnionOne(Set#Empty(): Set, 
+              $Box(#_System._tuple#2._#Make2($Box(t#0), $Box(_module.ChainingObject.tracking))))));
+    }
+
     newtype$check#3 := null;
     assume true;
     $rhs#5 := null;
-    havoc $ReferrersHeap;
+    if ($rhs#5 != null)
+    {
+        assume !Set#IsMember(readReferrers($ReferrersHeap, $rhs#5), 
+          $Box(#_System._tuple#2._#Make2($Box(t#0), $Box(_module.ChainingObject.tracking))));
+        $ReferrersHeap := updateReferrers($ReferrersHeap, 
+          $rhs#5, 
+          Set#UnionOne(readReferrers($ReferrersHeap, $rhs#5), 
+            $Box(#_System._tuple#2._#Make2($Box(t#0), $Box(_module.ChainingObject.tracking)))));
+    }
+
     $Heap := update($Heap, t#0, _module.ChainingObject.tracking, $Box($rhs#5));
     assume $IsGoodHeap($Heap);
     assume {:captureState "referrers.dfy(128,20)"} true;
@@ -4502,11 +4611,19 @@ implementation {:smt_option "smt.arith.solver", "2"} {:verboseName "ObjectFields
     assume true;
     assume true;
     assert {:id "id132"} $_ModifiesFrame[t#0, _module.ChainingObject.nontracking];
-    havoc $ReferrersHeap;
+    $oldRhs := $Unbox(read($Heap, t#0, _module.ChainingObject.nontracking)): ref;
+    if ($oldRhs != null)
+    {
+        $ReferrersHeap := updateReferrers($ReferrersHeap, 
+          $oldRhs, 
+          Set#Difference(readReferrers($ReferrersHeap, $oldRhs), 
+            Set#UnionOne(Set#Empty(): Set, 
+              $Box(#_System._tuple#2._#Make2($Box(t#0), $Box(_module.ChainingObject.nontracking))))));
+    }
+
     assert {:id "id133"} defass#t#0;
     assume true;
     $rhs#6 := t#0;
-    havoc $ReferrersHeap;
     $Heap := update($Heap, t#0, _module.ChainingObject.nontracking, $Box($rhs#6));
     assume $IsGoodHeap($Heap);
     assume {:captureState "referrers.dfy(130,20)"} true;
@@ -4584,11 +4701,29 @@ implementation {:smt_option "smt.arith.solver", "2"} {:verboseName "ObjectFields
     assume true;
     assume true;
     assert {:id "id150"} $_ModifiesFrame[u#0, _module.ChainingObject.x];
-    havoc $ReferrersHeap;
+    $oldRhs := $Unbox(read($Heap, u#0, _module.ChainingObject.x)): ref;
+    if ($oldRhs != null)
+    {
+        $ReferrersHeap := updateReferrers($ReferrersHeap, 
+          $oldRhs, 
+          Set#Difference(readReferrers($ReferrersHeap, $oldRhs), 
+            Set#UnionOne(Set#Empty(): Set, 
+              $Box(#_System._tuple#2._#Make2($Box(u#0), $Box(_module.ChainingObject.x))))));
+    }
+
     assert {:id "id151"} defass#t#0;
     assume true;
     $rhs#7 := t#0;
-    havoc $ReferrersHeap;
+    if ($rhs#7 != null)
+    {
+        assume !Set#IsMember(readReferrers($ReferrersHeap, $rhs#7), 
+          $Box(#_System._tuple#2._#Make2($Box(u#0), $Box(_module.ChainingObject.x))));
+        $ReferrersHeap := updateReferrers($ReferrersHeap, 
+          $rhs#7, 
+          Set#UnionOne(readReferrers($ReferrersHeap, $rhs#7), 
+            $Box(#_System._tuple#2._#Make2($Box(u#0), $Box(_module.ChainingObject.x)))));
+    }
+
     $Heap := update($Heap, u#0, _module.ChainingObject.x, $Box($rhs#7));
     assume $IsGoodHeap($Heap);
     assume {:captureState "referrers.dfy(137,10)"} true;
@@ -4614,11 +4749,29 @@ implementation {:smt_option "smt.arith.solver", "2"} {:verboseName "ObjectFields
     assume true;
     assume true;
     assert {:id "id162"} $_ModifiesFrame[u#0, _module.ChainingObject.x];
-    havoc $ReferrersHeap;
+    $oldRhs := $Unbox(read($Heap, u#0, _module.ChainingObject.x)): ref;
+    if ($oldRhs != null)
+    {
+        $ReferrersHeap := updateReferrers($ReferrersHeap, 
+          $oldRhs, 
+          Set#Difference(readReferrers($ReferrersHeap, $oldRhs), 
+            Set#UnionOne(Set#Empty(): Set, 
+              $Box(#_System._tuple#2._#Make2($Box(u#0), $Box(_module.ChainingObject.x))))));
+    }
+
     assert {:id "id163"} defass#u#0;
     assume true;
     $rhs#8 := u#0;
-    havoc $ReferrersHeap;
+    if ($rhs#8 != null)
+    {
+        assume !Set#IsMember(readReferrers($ReferrersHeap, $rhs#8), 
+          $Box(#_System._tuple#2._#Make2($Box(u#0), $Box(_module.ChainingObject.x))));
+        $ReferrersHeap := updateReferrers($ReferrersHeap, 
+          $rhs#8, 
+          Set#UnionOne(readReferrers($ReferrersHeap, $rhs#8), 
+            $Box(#_System._tuple#2._#Make2($Box(u#0), $Box(_module.ChainingObject.x)))));
+    }
+
     $Heap := update($Heap, u#0, _module.ChainingObject.x, $Box($rhs#8));
     assume $IsGoodHeap($Heap);
     assume {:captureState "referrers.dfy(140,10)"} true;
@@ -5172,6 +5325,7 @@ implementation {:smt_option "smt.arith.solver", "2"} {:verboseName "ChainingObje
   var this.nontracking: ref;
   var this.tracking: ref;
   var this.tail: ref;
+  var $oldRhs: ref;
   var newtype$check#2: ref;
   var newtype$check#3: ref;
   var newtype$check#4: ref;
@@ -5186,46 +5340,126 @@ implementation {:smt_option "smt.arith.solver", "2"} {:verboseName "ChainingObje
     // ----- assignment statement ----- C:\Users\mimayere\Documents\dafny\Source\IntegrationTests\TestFiles\LitTests\LitTest\referrers\referrers.dfy(103,7)
     assume true;
     assume true;
-    havoc $ReferrersHeap;
+    $oldRhs := $Unbox(read($Heap, this, _module.ChainingObject.x)): ref;
+    if ($oldRhs != null)
+    {
+        $ReferrersHeap := updateReferrers($ReferrersHeap, 
+          $oldRhs, 
+          Set#Difference(readReferrers($ReferrersHeap, $oldRhs), 
+            Set#UnionOne(Set#Empty(): Set, 
+              $Box(#_System._tuple#2._#Make2($Box(this), $Box(_module.ChainingObject.x))))));
+    }
+
     newtype$check#2 := null;
     assume true;
     this.x := null;
-    havoc $ReferrersHeap;
+    if (this.x != null)
+    {
+        assume !Set#IsMember(readReferrers($ReferrersHeap, this.x), 
+          $Box(#_System._tuple#2._#Make2($Box(this), $Box(_module.ChainingObject.x))));
+        $ReferrersHeap := updateReferrers($ReferrersHeap, 
+          this.x, 
+          Set#UnionOne(readReferrers($ReferrersHeap, this.x), 
+            $Box(#_System._tuple#2._#Make2($Box(this), $Box(_module.ChainingObject.x)))));
+    }
+
     assume {:captureState "referrers.dfy(103,13)"} true;
     // ----- assignment statement ----- C:\Users\mimayere\Documents\dafny\Source\IntegrationTests\TestFiles\LitTests\LitTest\referrers\referrers.dfy(104,7)
     assume true;
     assume true;
-    havoc $ReferrersHeap;
+    $oldRhs := $Unbox(read($Heap, this, _module.ChainingObject.y)): ref;
+    if ($oldRhs != null)
+    {
+        $ReferrersHeap := updateReferrers($ReferrersHeap, 
+          $oldRhs, 
+          Set#Difference(readReferrers($ReferrersHeap, $oldRhs), 
+            Set#UnionOne(Set#Empty(): Set, 
+              $Box(#_System._tuple#2._#Make2($Box(this), $Box(_module.ChainingObject.y))))));
+    }
+
     newtype$check#3 := null;
     assume true;
     this.y := null;
-    havoc $ReferrersHeap;
+    if (this.y != null)
+    {
+        assume !Set#IsMember(readReferrers($ReferrersHeap, this.y), 
+          $Box(#_System._tuple#2._#Make2($Box(this), $Box(_module.ChainingObject.y))));
+        $ReferrersHeap := updateReferrers($ReferrersHeap, 
+          this.y, 
+          Set#UnionOne(readReferrers($ReferrersHeap, this.y), 
+            $Box(#_System._tuple#2._#Make2($Box(this), $Box(_module.ChainingObject.y)))));
+    }
+
     assume {:captureState "referrers.dfy(104,13)"} true;
     // ----- assignment statement ----- C:\Users\mimayere\Documents\dafny\Source\IntegrationTests\TestFiles\LitTests\LitTest\referrers\referrers.dfy(105,14)
     assume true;
     assume true;
-    havoc $ReferrersHeap;
+    $oldRhs := $Unbox(read($Heap, this, _module.ChainingObject.tracking)): ref;
+    if ($oldRhs != null)
+    {
+        $ReferrersHeap := updateReferrers($ReferrersHeap, 
+          $oldRhs, 
+          Set#Difference(readReferrers($ReferrersHeap, $oldRhs), 
+            Set#UnionOne(Set#Empty(): Set, 
+              $Box(#_System._tuple#2._#Make2($Box(this), $Box(_module.ChainingObject.tracking))))));
+    }
+
     newtype$check#4 := null;
     assume true;
     this.tracking := null;
-    havoc $ReferrersHeap;
+    if (this.tracking != null)
+    {
+        assume !Set#IsMember(readReferrers($ReferrersHeap, this.tracking), 
+          $Box(#_System._tuple#2._#Make2($Box(this), $Box(_module.ChainingObject.tracking))));
+        $ReferrersHeap := updateReferrers($ReferrersHeap, 
+          this.tracking, 
+          Set#UnionOne(readReferrers($ReferrersHeap, this.tracking), 
+            $Box(#_System._tuple#2._#Make2($Box(this), $Box(_module.ChainingObject.tracking)))));
+    }
+
     assume {:captureState "referrers.dfy(105,20)"} true;
     // ----- assignment statement ----- C:\Users\mimayere\Documents\dafny\Source\IntegrationTests\TestFiles\LitTests\LitTest\referrers\referrers.dfy(106,17)
     assume true;
     assume true;
-    havoc $ReferrersHeap;
+    $oldRhs := $Unbox(read($Heap, this, _module.ChainingObject.nontracking)): ref;
+    if ($oldRhs != null)
+    {
+        $ReferrersHeap := updateReferrers($ReferrersHeap, 
+          $oldRhs, 
+          Set#Difference(readReferrers($ReferrersHeap, $oldRhs), 
+            Set#UnionOne(Set#Empty(): Set, 
+              $Box(#_System._tuple#2._#Make2($Box(this), $Box(_module.ChainingObject.nontracking))))));
+    }
+
     newtype$check#5 := null;
     assume true;
     this.nontracking := null;
-    havoc $ReferrersHeap;
     assume {:captureState "referrers.dfy(106,23)"} true;
     // ----- assignment statement ----- C:\Users\mimayere\Documents\dafny\Source\IntegrationTests\TestFiles\LitTests\LitTest\referrers\referrers.dfy(107,10)
     assume true;
     assume true;
-    havoc $ReferrersHeap;
+    $oldRhs := $Unbox(read($Heap, this, _module.ChainingObject.tail)): ref;
+    if ($oldRhs != null)
+    {
+        $ReferrersHeap := updateReferrers($ReferrersHeap, 
+          $oldRhs, 
+          Set#Difference(readReferrers($ReferrersHeap, $oldRhs), 
+            Set#UnionOne(Set#Empty(): Set, 
+              $Box(#_System._tuple#2._#Make2($Box(this), $Box(_module.ChainingObject.tail))))));
+    }
+
     assume true;
     this.tail := chained_test#0;
-    havoc $ReferrersHeap;
+    if (this.tail != null)
+    {
+        assume !Set#IsMember(readReferrers($ReferrersHeap, this.tail), 
+          $Box(#_System._tuple#2._#Make2($Box(this), $Box(_module.ChainingObject.tail))));
+        $ReferrersHeap := updateReferrers($ReferrersHeap, 
+          this.tail, 
+          Set#UnionOne(readReferrers($ReferrersHeap, this.tail), 
+            $Box(#_System._tuple#2._#Make2($Box(this), $Box(_module.ChainingObject.tail)))));
+    }
+
     assume {:captureState "referrers.dfy(107,24)"} true;
     // ----- new; ----- C:\Users\mimayere\Documents\dafny\Source\IntegrationTests\TestFiles\LitTests\LitTest\referrers\referrers.dfy(102,3)
     assume this != null && $Is(this, Tclass._module.ChainingObject?());
